Stratego/Examples/Arithmetic.thy
@@ -1,0 +1,126 @@
+theory Arithmetic
+  imports "HOL-Library.Finite_Map" "HOL-Library.Monad_Syntax"
+begin
+
+
+subsection "Example: Simple Arithmetic Rewrites"
+
+datatype (discs_sels) Arithmetic =
+  Add Arithmetic Arithmetic |
+  Sub Arithmetic Arithmetic |
+  UMinus Arithmetic |
+  Number int |
+  Variable string
+
+fun compatible :: "('a, 'b) fmap \<Rightarrow> ('a, 'b) fmap \<Rightarrow> bool" where
+  "compatible s1 s2 = (\<forall>x \<in> fset (fmdom s1) . fmlookup s2 x \<noteq> None \<longrightarrow> fmlookup s1 x = fmlookup s2 x)"
+
+fun union :: "(('a, 'b) fmap) option \<Rightarrow> (('a, 'b) fmap) option \<Rightarrow> (('a, 'b) fmap) option" where
+  "union s1 s2 = do {
+    s1' <- s1;
+    s2' <- s2;
+    if compatible s1' s2' then Some (s1' ++\<^sub>f s2') else None
+  }"
+
+fun match_Arithmetic :: "Arithmetic \<Rightarrow> Arithmetic \<Rightarrow> ((string, Arithmetic) fmap) option" where
+  "match_Arithmetic (Add x y) (Add x' y') = 
+    union (match_Arithmetic x x') (match_Arithmetic y y')" |
+  "match_Arithmetic (Sub x y) (Sub x' y') =
+    union (match_Arithmetic x x') (match_Arithmetic y y')" |
+  "match_Arithmetic (UMinus x) (UMinus x') =
+    (match_Arithmetic x x')" |
+  "match_Arithmetic (Number v) (Number v') = (if v = v' then Some (fmempty) else None)" |
+  "match_Arithmetic (Variable v) e = Some (fmupd v e fmempty)" |
+  "match_Arithmetic _ _ = None"
+
+fun varof_Arithmetic :: "Arithmetic \<Rightarrow> string option" where
+  "varof_Arithmetic (Variable s) = Some s" |
+  "varof_Arithmetic _ = None"
+
+fun var_Arithmetic :: "string \<Rightarrow> Arithmetic" where
+  "var_Arithmetic v = Variable v"
+
+fun rewrite_Arithmetic :: "(Arithmetic \<Rightarrow> Arithmetic) \<Rightarrow> Arithmetic \<Rightarrow> Arithmetic" where
+  "rewrite_Arithmetic f (Add x y) = f (Add (rewrite_Arithmetic f x) (rewrite_Arithmetic f y))" |
+  "rewrite_Arithmetic f (Sub x y) = f (Sub (rewrite_Arithmetic f x) (rewrite_Arithmetic f y))" |
+  "rewrite_Arithmetic f (UMinus x) = f (UMinus (rewrite_Arithmetic f x))" |
+  "rewrite_Arithmetic f (Number v) = f (Number v)" |
+  "rewrite_Arithmetic f (Variable s) = f (Variable s)"
+
+fun subexprs_Arithmetic :: "Arithmetic \<Rightarrow> Arithmetic list" where
+  "subexprs_Arithmetic (Add x y) = [x, y]" |
+  "subexprs_Arithmetic (Sub x y) = [x, y]" |
+  "subexprs_Arithmetic (UMinus x) = [x]" |
+  "subexprs_Arithmetic (Number v) = []" |
+  "subexprs_Arithmetic (Variable s) = []"
+
+fun chain_Arithmetic :: "(Arithmetic \<Rightarrow> nat \<Rightarrow> (nat \<times> Arithmetic)) \<Rightarrow> Arithmetic \<Rightarrow> nat \<Rightarrow> (nat \<times> Arithmetic)" where
+  "chain_Arithmetic f (Add x y) n =
+    (let (n', x') = f x n in
+    (let (n'', y') = f y n' in
+      (n'', Add x' y')))" |
+  "chain_Arithmetic f (Sub x y) n =
+    (let (n', x') = f x n in
+    (let (n'', y') = f y n' in
+      (n'', Sub x' y')))" |
+  "chain_Arithmetic f (UMinus x) n =
+    (let (n', x') = f x n in
+      (n', UMinus x'))" |
+  "chain_Arithmetic f (Number v) n = (n, (Number v))" |
+  "chain_Arithmetic f (Variable s) n = (n, (Variable s))"
+
+datatype ArithmeticCondition =
+  IsSub Arithmetic |
+  IsNumber Arithmetic
+
+fun eval_condition :: "ArithmeticCondition \<Rightarrow> bool option" where
+  "eval_condition (IsSub (Sub x y)) = Some True" |
+  "eval_condition (IsNumber (Number v)) = Some True" |
+  "eval_condition (IsSub (Variable v)) = None" |
+  "eval_condition (IsNumber (Variable v)) = None" |
+  "eval_condition _ = Some False"
+
+fun ground_condition :: "ArithmeticCondition \<Rightarrow> (string \<rightharpoonup> Arithmetic) \<Rightarrow> ArithmeticCondition" where
+  "ground_condition (IsSub (Variable v)) f = (case f v of 
+                                              Some v' \<Rightarrow> (IsSub v') |
+                                              None \<Rightarrow> (IsSub (Variable v)))" |
+  "ground_condition (IsNumber (Variable v)) f = (case f v of 
+                                              Some v' \<Rightarrow> (IsNumber v') |
+                                              None \<Rightarrow> (IsNumber (Variable v)))" |
+  "ground_condition e f = e"
+
+fun is_ground_condition :: "ArithmeticCondition \<Rightarrow> bool" where
+  "is_ground_condition (IsSub e) = (\<not>(is_Variable e))" |
+  "is_ground_condition (IsNumber e) = (\<not>(is_Variable e))"
+
+datatype Transformer =
+  UnaryMinus Arithmetic |
+  Plus Arithmetic Arithmetic |
+  Result Arithmetic
+
+fun eval_transformer :: "Transformer \<Rightarrow> Arithmetic option" where
+  "eval_transformer (UnaryMinus (Number x)) = Some (Number (-x))" |
+  "eval_transformer (Plus (Number x) (Number y)) = Some (Number (plus x y))" |
+  "eval_transformer (Result a) = Some a" |
+  "eval_transformer _ = None"
+
+fun ground_transformer :: "Transformer \<Rightarrow> (string \<rightharpoonup> Arithmetic) \<Rightarrow> Transformer" where
+  "ground_transformer (UnaryMinus (Variable v)) f = (case f v of 
+                                              Some v' \<Rightarrow> (UnaryMinus v') |
+                                              None \<Rightarrow> (UnaryMinus (Variable v)))" |
+  "ground_transformer (Plus (Variable x) (Variable y)) f = (case f x of 
+                                              Some x' \<Rightarrow> (
+                                                case f y of Some y' \<Rightarrow> (Plus x' y')
+                                                            | None \<Rightarrow> (Plus (Variable x) (Variable y)))
+                                              | None \<Rightarrow> (Plus (Variable x) (Variable y)))" |
+  "ground_transformer (Result (Variable v)) f = (case f v of 
+                                              Some v' \<Rightarrow> (Result v') |
+                                              None \<Rightarrow> (Result (Variable v)))" |
+  "ground_transformer e f = e"
+
+fun is_ground_transformer :: "Transformer \<Rightarrow> bool" where
+  "is_ground_transformer (UnaryMinus e) = is_Variable e" |
+  "is_ground_transformer (Plus e1 e2) = (is_Variable e1 \<or> is_Variable e2)" |
+  "is_ground_transformer (Result e) = is_Variable e"
+
+end
