Stratego/Examples/ArithmeticExample.thy
@@ -1,0 +1,258 @@
+theory ArithmeticExample
+  imports Arithmetic "../JavaExport"
+begin
+
+context Rewritable begin
+termination match_pattern sorry
+end
+
+setup \<open>Locale_Code.open_block\<close>
+interpretation Arithmetic: Rewritable
+  size_Arithmetic
+  
+  eval_condition ground_condition is_ground_condition
+  eval_transformer ground_transformer is_ground_transformer
+
+  subexprs_Arithmetic chain_Arithmetic rewrite_Arithmetic
+  match_Arithmetic
+
+  varof_Arithmetic var_Arithmetic
+proof
+  fix c :: ArithmeticCondition
+  fix a' a :: "(string \<rightharpoonup> Arithmetic)"
+  assume sub: "a' \<subseteq>\<^sub>m a"
+  assume ground: "is_ground_condition (ground_condition c a')"
+  show "ground_condition c a' = ground_condition c a"
+    using sub ground 
+    apply (induction c a rule: ground_condition.induct)
+    defer defer apply simp+
+    subgoal premises prem for e f
+    proof (cases "a' e")
+      case None
+      then have "\<not>(is_ground_condition (case a' e of None \<Rightarrow> IsSub (Variable e) | Some x \<Rightarrow> IsSub x))"
+        by simp
+      then show ?thesis using prem by blast
+    next
+      case (Some a)
+      then have "a' e = f e" using prem(1)
+        by (metis domIff map_le_def option.distinct(1))
+      then show ?thesis by simp
+    qed
+    apply simp
+    subgoal premises prem for e f
+    proof (cases "a' e")
+      case None
+      then have "\<not>(is_ground_condition (case a' e of None \<Rightarrow> IsNumber (Variable e) | Some x \<Rightarrow> IsNumber x))"
+        by simp
+      then show ?thesis using prem by blast
+    next
+      case (Some a)
+      then have "a' e = f e" using prem(1)
+        by (metis domIff map_le_def option.distinct(1))
+      then show ?thesis by simp
+    qed
+    done
+next
+  fix e :: Arithmetic
+  show "\<forall>e' \<in> set (subexprs_Arithmetic e). size_Arithmetic e > size_Arithmetic e'"
+    by (cases e; simp)
+next
+  fix f :: "Arithmetic \<Rightarrow> Arithmetic"
+  fix e :: Arithmetic
+  show "map f (subexprs_Arithmetic e) = subexprs_Arithmetic (snd (chain_Arithmetic (\<lambda>e a. (plus a 1, f e)) e 0))"
+    by (cases e; simp)
+next
+  fix f :: "Arithmetic \<Rightarrow> Arithmetic"
+  fix e :: Arithmetic
+  show "length (subexprs_Arithmetic e) = fst (chain_Arithmetic (\<lambda>e a. (plus a 1, f e)) e 0)"
+    by (cases e; simp)
+next
+  fix c :: "ArithmeticCondition"
+  have lhs: "eval_condition c = None \<Longrightarrow> (\<not> is_ground_condition c)"
+  subgoal premises e
+  proof (cases c)
+    case (IsSub x1)
+    then show ?thesis using e by (cases x1; auto) 
+  next
+    case (IsNumber x2)
+    then show ?thesis using e by (cases x2; auto)
+  qed
+  done
+  have rhs: "(\<not> is_ground_condition c) \<Longrightarrow> eval_condition c = None"
+  subgoal premises e
+  proof (cases c)
+    case (IsSub x1)
+    then show ?thesis using e by (cases x1; auto) 
+  next
+    case (IsNumber x2)
+    then show ?thesis using e by (cases x2; auto)
+  qed
+  done
+  from lhs rhs show "eval_condition c = None \<equiv> (\<not> is_ground_condition c)"
+    by linarith
+qed
+setup \<open>Locale_Code.close_block\<close>
+
+
+
+subsubsection \<open>Example: Match Pattern\<close>
+
+definition "join = Arithmetic.join"
+definition "generate = Arithmetic.generate"
+definition "match_pattern = Arithmetic.match_pattern"
+definition "optimized_export = Arithmetic.optimized_export"
+definition "var = var_Arithmetic"
+
+export_code "optimized_export" checking SML
+
+
+export_code "match_pattern" checking SML
+
+value "match_pattern
+(Sub (Add (Variable ''x'') (Variable ''y'')) (Variable ''y''))
+''e'' ({|''e''|}, Map.empty)"
+text \<open>@{value "match_pattern
+(Sub (Add (Variable ''x'') (Variable ''y'')) (Variable ''y''))
+''e'' ({|''e''|}, Map.empty)"}\<close>
+
+value "match_pattern
+(Sub 
+    (Add 
+        (Sub (Variable ''x'') (Variable ''x''))
+        (Sub (Variable ''y'') (Variable ''x'')))
+    (Variable ''y''))
+''e'' ({|''e''|}, Map.empty)"
+text \<open>@{value "match_pattern
+(Sub 
+    (Add 
+        (Sub (Variable ''x'') (Variable ''x''))
+        (Sub (Variable ''y'') (Variable ''x'')))
+    (Variable ''y''))
+''e'' ({|''e''|}, Map.empty)"}\<close>
+
+definition Identity where
+  "Identity = generate 
+    (Add
+      (var ''x'')
+      (Number 0))
+    (Result (var ''x''))"
+
+value "Identity"
+text "@{value[display] \<open>Identity\<close>}"
+value "optimized_export Identity"
+text "@{value[display] \<open>optimized_export Identity\<close>}"
+
+text \<open>@{text "const x + const y \<longrightarrow> const (x + y)"}\<close>
+definition Evaluate where
+  "Evaluate = generate 
+    (Add
+      (var ''x'')
+      (var ''y''))
+    (Plus (var ''x'') (var ''y''))"
+(* doesn't support constant evaluation *)
+value "Evaluate"
+value "(optimized_export (Evaluate))"
+
+text \<open>@{text "const x + y \<longrightarrow> y + const x when NotConst y"}\<close>
+definition LeftConst where
+  "LeftConst = generate 
+    (Add
+      (var ''x'')
+      (var ''y''))
+    (Plus (var ''y'') (var ''x''))"
+value "LeftConst"
+
+value "(choice [LeftConst, Evaluate, Identity])"
+text "@{value[display] \<open>choice [LeftConst, Evaluate, Identity]\<close>}"
+value "(optimized_export (choice [LeftConst, Evaluate, Identity]))"
+text "@{value[display] \<open>(optimized_export (choice [LeftConst, Evaluate, Identity]))\<close>}"
+value "(optimized_export (optimized_export (choice [LeftConst, Evaluate, Identity])))"
+text "@{value[display] \<open>(optimized_export (optimized_export (choice [LeftConst, Evaluate, Identity])))\<close>}"
+
+
+
+fun class_of_term_Arithmetic :: "Arithmetic \<Rightarrow> string" where
+  "class_of_term_Arithmetic (Add x y) = ''AddNode''" |
+  "class_of_term_Arithmetic (Sub x y) = ''SubNode''" |
+  "class_of_term_Arithmetic (UMinus x) = ''UnaryMinusNode''" |
+  "class_of_term_Arithmetic (Number v) = ''ConstantNode''" |
+  "class_of_term_Arithmetic (Variable s) = ''VariableNode''"
+
+datatype JavaCheck =
+  CallMethod1 |
+  CallMethod2 |
+  MethodCall string string |
+  Construct string "JavaCheck list" |
+  VariableExpr string
+
+instantiation "JavaCheck" :: JavaExpression
+begin
+fun expToJava_JavaCheck where
+  "expToJava_JavaCheck CallMethod1 = ''I'm asserting you're a number''" |
+  "expToJava_JavaCheck CallMethod2 = ''I'm asserting you're a subnode''" |
+  "expToJava_JavaCheck (MethodCall ob m) = ob @ ''.'' @ m @ ''()''" |
+  "expToJava_JavaCheck (Construct class args) = ''new '' @ class @ ''('' @ param_list (map expToJava_JavaCheck args) @ '')''" |
+  "expToJava_JavaCheck (VariableExpr v) = v"
+instance ..
+end
+
+fun generate_condition_Arithmetic :: "ArithmeticCondition \<Rightarrow> JavaCheck" where
+  "generate_condition_Arithmetic (IsSub e) = CallMethod2" |
+  "generate_condition_Arithmetic (IsNumber e) = CallMethod1"
+
+fun generate_Arithmetic :: "Arithmetic \<Rightarrow> JavaCheck" where
+  "generate_Arithmetic (Add x y) = Construct ''AddNode'' (map generate_Arithmetic [x, y])" |
+  "generate_Arithmetic (Sub x y) = Construct ''SubNode'' (map generate_Arithmetic [x, y])" |
+  "generate_Arithmetic (UMinus x) = Construct ''UnaryMinusNode'' (map generate_Arithmetic [x])" |
+  "generate_Arithmetic (Number v) = Construct ''ConstantNode'' []" |
+  "generate_Arithmetic (Variable s) = VariableExpr s"
+
+fun generate_result_Arithmetic :: "Transformer \<Rightarrow> JavaCheck" where
+  "generate_result_Arithmetic (UnaryMinus e) = CallMethod1" |
+  "generate_result_Arithmetic (Plus e1 e2) = CallMethod2" |
+  "generate_result_Arithmetic (Result e) = generate_Arithmetic e"
+
+fun generate_access_Arithmetic :: "VarName \<Rightarrow> Arithmetic \<Rightarrow> JavaCheck list" where
+  "generate_access_Arithmetic v (Add x y) = 
+    [(MethodCall v ''getX''),
+     (MethodCall v ''getY'')]" |
+  "generate_access_Arithmetic v (Sub x y) = 
+    [(MethodCall v ''getX''),
+     (MethodCall v ''getY'')]" |
+  "generate_access_Arithmetic v (UMinus x) = [(MethodCall v ''getValue'')]" |
+  "generate_access_Arithmetic v (Number val) = []" |
+  "generate_access_Arithmetic v (Variable s) = []"
+
+setup \<open>Locale_Code.open_block\<close>
+interpretation Arithmetic: JavaTarget
+  size_Arithmetic
+  "eval_condition"
+  "ground_condition"
+  "is_ground_condition"
+  "eval_transformer"
+  "ground_transformer"
+  "is_ground_transformer"
+  subexprs_Arithmetic
+  chain_Arithmetic
+  rewrite_Arithmetic
+  match_Arithmetic
+  varof_Arithmetic
+  var_Arithmetic
+  
+  class_of_term_Arithmetic
+  generate_condition_Arithmetic
+  generate_result_Arithmetic
+  generate_access_Arithmetic
+  by standard
+setup \<open>Locale_Code.close_block\<close>
+
+definition "export_rules = Arithmetic.export_rules"
+value "export_rules"
+
+value "export_rules (optimized_export (choice [Identity, Evaluate]))"
+value "export_rules (optimized_export (Identity \<then> Evaluate))"
+
+value "statementToJava 0 (export_rules (optimized_export (choice [Identity, Evaluate])))"
+
+
+end
