Stratego/Examples/ArithmeticStratego.thy
@@ -1,0 +1,184 @@
+theory ArithmeticStratego
+  imports Arithmetic "../Stratego"
+begin
+
+setup \<open>Locale_Code.open_block\<close>
+interpretation Arithmetic: Rewritable
+  size_Arithmetic
+  
+  eval_condition ground_condition is_ground_condition
+  eval_transformer ground_transformer is_ground_transformer
+
+  subexprs_Arithmetic chain_Arithmetic rewrite_Arithmetic
+  match_Arithmetic
+
+  varof_Arithmetic var_Arithmetic
+proof
+  fix c :: ArithmeticCondition
+  fix a' a :: "(string \<rightharpoonup> Arithmetic)"
+  assume sub: "a' \<subseteq>\<^sub>m a"
+  assume ground: "is_ground_condition (ground_condition c a')"
+  show "ground_condition c a' = ground_condition c a"
+    using sub ground 
+    apply (induction c a rule: ground_condition.induct)
+    defer defer apply simp+
+    subgoal premises prem for e f
+    proof (cases "a' e")
+      case None
+      then have "\<not>(is_ground_condition (case a' e of None \<Rightarrow> IsSub (Variable e) | Some x \<Rightarrow> IsSub x))"
+        by simp
+      then show ?thesis using prem by blast
+    next
+      case (Some a)
+      then have "a' e = f e" using prem(1)
+        by (metis domIff map_le_def option.distinct(1))
+      then show ?thesis by simp
+    qed
+    apply simp
+    subgoal premises prem for e f
+    proof (cases "a' e")
+      case None
+      then have "\<not>(is_ground_condition (case a' e of None \<Rightarrow> IsNumber (Variable e) | Some x \<Rightarrow> IsNumber x))"
+        by simp
+      then show ?thesis using prem by blast
+    next
+      case (Some a)
+      then have "a' e = f e" using prem(1)
+        by (metis domIff map_le_def option.distinct(1))
+      then show ?thesis by simp
+    qed
+    done
+next
+  fix e :: Arithmetic
+  show "\<forall>e' \<in> set (subexprs_Arithmetic e). size_Arithmetic e > size_Arithmetic e'"
+    by (cases e; simp)
+next
+  fix f :: "Arithmetic \<Rightarrow> Arithmetic"
+  fix e :: Arithmetic
+  show "map f (subexprs_Arithmetic e) = subexprs_Arithmetic (snd (chain_Arithmetic (\<lambda>e a. (plus a 1, f e)) e 0))"
+    by (cases e; simp)
+next
+  fix f :: "Arithmetic \<Rightarrow> Arithmetic"
+  fix e :: Arithmetic
+  show "length (subexprs_Arithmetic e) = fst (chain_Arithmetic (\<lambda>e a. (plus a 1, f e)) e 0)"
+    by (cases e; simp)
+next
+  fix c :: "ArithmeticCondition"
+  have lhs: "eval_condition c = None \<Longrightarrow> (\<not> is_ground_condition c)"
+  subgoal premises e
+  proof (cases c)
+    case (IsSub x1)
+    then show ?thesis using e by (cases x1; auto) 
+  next
+    case (IsNumber x2)
+    then show ?thesis using e by (cases x2; auto)
+  qed
+  done
+  have rhs: "(\<not> is_ground_condition c) \<Longrightarrow> eval_condition c = None"
+  subgoal premises e
+  proof (cases c)
+    case (IsSub x1)
+    then show ?thesis using e by (cases x1; auto) 
+  next
+    case (IsNumber x2)
+    then show ?thesis using e by (cases x2; auto)
+  qed
+  done
+  from lhs rhs show "eval_condition c = None \<equiv> (\<not> is_ground_condition c)"
+    by linarith
+qed
+setup \<open>Locale_Code.close_block\<close>
+
+subsubsection "Stratego Rules"
+
+definition "eval = Arithmetic.eval"
+definition "var = var_Arithmetic"
+
+notation Arithmetic.conditional_rewrite_to ("_ \<rightarrow> _ where _")
+
+type_synonym StrategyRule = "(Arithmetic, ArithmeticCondition, Transformer) Strategy"
+
+export_code "eval" checking SML
+
+definition RedundantAdd :: "StrategyRule" where
+  "RedundantAdd = ((Add (var ''b'') (Number 0)) \<rightarrow> (var ''b''))"
+
+value "eval (RedundantAdd) ((Add (Number 10) (Number 10)), fmempty)"
+
+definition RedundantSub :: "StrategyRule" where
+  "RedundantSub = ((Sub (var ''a'') (Number 0)) \<rightarrow> (var ''a'') where condition (IsSub (var ''a'')))"
+
+value "eval (RedundantSub) ((Sub (Number 10) (Number 0)), fmempty)"
+value "eval (RedundantSub) ((Sub (Sub (Number 100) (Number 1000)) (Number 0)), fmempty)"
+
+
+definition ShiftConstRight :: "StrategyRule" where
+  "ShiftConstRight = 
+    ((Add (var ''a'') (var ''b'')) \<rightarrow> (Add (var ''b'') (var ''a''))
+      where ((var ''a'')!; not (Number 0?)))"
+
+definition ShiftConstRight2 :: "StrategyRule" where
+  "ShiftConstRight2 = 
+    ((Add (var ''a'') (var ''b'')) \<rightarrow> (Add (var ''b'') (var ''a''))
+      where (condition (IsNumber (var ''a''))))"
+
+definition EvalMinus :: "StrategyRule" where
+  "EvalMinus = 
+    ((UMinus (Variable ''a'')) \<rightarrow> ((Variable ''b''))
+      where (condition (IsNumber (Variable ''a'')); func (UnaryMinus (Variable ''a'')); (Variable ''b'')?))"
+
+definition EvalMinus1 :: "StrategyRule" where
+  "EvalMinus1 =
+    (UMinus (Variable ''a'')) \<rightarrow> Variable ''b''
+      where (condition (IsNumber (Variable ''a'')); (Variable ''b'') := (func (UnaryMinus (Variable ''a''))))"
+
+definition EvalAdd :: "StrategyRule" where
+  "EvalAdd =
+    ((Add (Variable ''a'') (Variable ''b'')) \<rightarrow> ((Variable ''c''))
+      where (
+        (condition (IsNumber (Variable ''a'')));
+        (condition (IsNumber (Variable ''a'')));
+        ((Variable ''c'') := (func (Plus (Variable ''a'') (Variable ''b''))))
+      ))"
+
+subsubsection "Rewrite Application"
+
+text "
+The combination of @{term RedundantAdd} and @{term RedundantSub}
+provides us a rule that will eliminate zero in either add or sub expressions.
+It is defined as @{term \<open>RedundantAdd <+ RedundantSub\<close>}.
+The expanded version of this rule is:
+
+@{value \<open>RedundantAdd <+ RedundantSub\<close>}"
+
+\<comment> \<open>Failing to apply the rule\<close>
+value "eval (RedundantAdd <+ RedundantSub) ((Add (Number 10) (Number 10)), fmempty)"
+text \<open>@{value "eval (RedundantAdd <+ RedundantSub) ((Add (Number 10) (Number 10)), fmempty)"}\<close>
+
+\<comment> \<open>Successful application\<close>
+value "eval (RedundantAdd <+ RedundantSub) ((Add (Number 10) (Number 0)), fmempty)"
+text \<open>@{value "eval (RedundantAdd <+ RedundantSub) ((Add (Number 10) (Number 0)), fmempty)"}\<close>
+
+\<comment> \<open>Successful application in the second rule\<close>
+value "eval (RedundantSub <+ RedundantAdd) ((Add (Number 10) (Number 0)), fmempty)"
+text \<open>@{value "eval (RedundantSub <+ RedundantAdd) ((Add (Number 10) (Number 0)), fmempty)"}\<close>
+
+value "ShiftConstRight"
+value "eval ShiftConstRight ((Add (Number 0) (Number 10)), fmempty)"
+value "eval ShiftConstRight ((Add (Number 10) (Add (Number 10) (Number 20))), fmempty)"
+value "eval ShiftConstRight ((Add (Number 10) (Number 120)), fmempty)"
+
+value "eval ShiftConstRight2 ((Add (Number 0) (Number 10)), fmempty)"
+value "eval ShiftConstRight2 ((Add (Number 10) (Add (Number 10) (Number 20))), fmempty)"
+value "eval ShiftConstRight2 ((Add (Number 10) (Number 120)), fmempty)"
+
+value "eval EvalMinus ((UMinus (Number 10)), fmempty)"
+value "eval EvalMinus ((UMinus (Add (Number 10) (Number 10))), fmempty)"
+text \<open>@{value "eval EvalMinus ((UMinus (Number 10)), fmempty)"}\<close>
+
+value "eval EvalAdd ((UMinus (Number 10)), fmempty)"
+value "eval EvalAdd ((Add (Number 10) (Number 10)), fmempty)"
+text \<open>@{value "eval EvalAdd ((Add (Number 10) (Number 10)), fmempty)"}\<close>
+
+
+end
