Stratego/Stratego.thy
@@ -1,60 +1,7 @@
 section "Stratego"
 theory Stratego
-  imports Main "HOL-Library.Finite_Map" "HOL-Library.Word" Locale_Code.Locale_Code "HOL-Library.Monad_Syntax"
+  imports Rewritable
 begin
-
-text \<open>
-We generalize the concept of a datatype that can be rewritten using Stratego
-using the @{term Rewritable} class.
-
-\begin{description}
-  \item[rewrite] Provides a mechanism for rewriting the AST given 
-    a leaf to leaf function applied to the root of the AST and returning the transformed AST.
-  \item[match] Given two ASTs, return a binding of variables of the first AST to the concrete second AST
-    if it matches, else return None.
-  \item[varof] Extract the identifier of the given AST if it is a variable, else None.
-  \item[var] Construct an AST to represent the variable given.
-\end{description}
-\<close>
-
-locale Groundable =
-  fixes eval :: "'a \<Rightarrow> 'c option"
-  fixes ground :: "'a \<Rightarrow> (string \<rightharpoonup> 'b) \<Rightarrow> 'a"
-  fixes is_ground :: "'a \<Rightarrow> bool"
-
-type_synonym 'e Binding = "(string, 'e) fmap"
-
-locale Rewritable =
-  size size +
-  Groundable eval_condition ground_condition is_ground_condition +
-  Groundable eval_result ground_result is_ground_result
-  for size :: "'a \<Rightarrow> nat"
-  and eval_condition :: "'b \<Rightarrow> bool option"
-  and ground_condition :: "'b \<Rightarrow> (string \<rightharpoonup> 'a) \<Rightarrow> 'b"
-  and is_ground_condition :: "'b \<Rightarrow> bool"
-  and eval_result :: "'c \<Rightarrow> 'a option"
-  and ground_result :: "'c \<Rightarrow> (string \<rightharpoonup> 'a) \<Rightarrow> 'c"
-  and is_ground_result :: "'c \<Rightarrow> bool"
- +
-  fixes subexprs :: "'a \<Rightarrow> 'a list"
-  fixes chain :: "('a \<Rightarrow> nat \<Rightarrow> (nat \<times> 'a)) \<Rightarrow> 'a \<Rightarrow> nat \<Rightarrow> (nat \<times> 'a)"
-  fixes rewrite :: "('a \<Rightarrow> 'a) \<Rightarrow> 'a \<Rightarrow> 'a"
-  fixes match_term :: "'a \<Rightarrow> 'a \<Rightarrow> ((string, 'a) fmap) option"
-  fixes varof :: "'a \<Rightarrow> string option"
-  fixes var :: "string \<Rightarrow> 'a"
-
-  (*fixes eval_condition :: "'b \<Rightarrow> bool"
-  fixes ground_condition :: "'b \<Rightarrow> (string \<rightharpoonup> 'a) \<Rightarrow> 'b option"
-
-  fixes transform :: "'c \<Rightarrow> 'a \<Rightarrow> 'a option"*)
-  assumes "a' \<subseteq>\<^sub>m a \<Longrightarrow> is_ground_condition (ground_condition c a') \<Longrightarrow> ground_condition c a' = ground_condition c a"
-  assumes shrinks: "\<forall>e' \<in> set (subexprs e). size e > size e'"
-  assumes "map f (subexprs e) = subexprs (snd (chain (\<lambda>e a. (plus a 1, f e)) e 0))"
-  assumes "length (subexprs e) = fst (chain (\<lambda>e a. (plus a 1, f e)) e 0)"
-  assumes "eval_condition c = None \<equiv> \<not>(is_ground_condition c)"
-begin
-(*fun rewrite :: "('a \<Rightarrow> 'a) \<Rightarrow> 'a \<Rightarrow> 'a" where
-  "rewrite f xs = snd (chain (\<lambda>e a. (plus a 1, f e)) xs (0::nat))"*)
 
 no_notation plus (infixl "+" 65)
 no_notation less ("(_/ < _)"  [51, 51] 50)
@@ -83,13 +30,6 @@ abbreviation rewrite_to :: "'a \<Rightarrow> 'a \<Rightarrow> ('a, 'b, 'c) Strat
   ("_ \<rightarrow> _") where
   "(s1 \<rightarrow> s2) \<equiv> s1?; s2!"
 
-abbreviation "wheref" :: "('a, 'b, 'c) Strategy \<Rightarrow> ('a, 'b, 'c) Strategy" where
-  "wheref x \<equiv> var ''_''?; x; var ''_''!"
-
-abbreviation conditional_rewrite_to :: "'a \<Rightarrow> 'a \<Rightarrow> ('a, 'b, 'c) Strategy \<Rightarrow> ('a, 'b, 'c) Strategy"
-  ("_ \<rightarrow> _ where _") where 
-  "s1 \<rightarrow> s2 where s3 \<equiv> s1?; wheref s3; s2!"
-
 abbreviation not :: "('a, 'b, 'c) Strategy \<Rightarrow> ('a, 'b, 'c) Strategy" where 
   "not s \<equiv> (s < fail + id)"
 
@@ -106,6 +46,14 @@ abbreviation assign :: "'a \<Rightarrow> ('a, 'b, 'c) Strategy \<Rightarrow> ('a
   \<comment> \<open>This should be trm => vars but this doesn't work well in Isabelle so swapped argument order.\<close>
   "vars := trm \<equiv> trm; vars?"
 
+context Rewritable begin
+
+abbreviation "wheref" :: "('a, 'b, 'c) Strategy \<Rightarrow> ('a, 'b, 'c) Strategy" where
+  "wheref x \<equiv> var ''_''?; x; var ''_''!"
+
+abbreviation conditional_rewrite_to :: "'a \<Rightarrow> 'a \<Rightarrow> ('a, 'b, 'c) Strategy \<Rightarrow> ('a, 'b, 'c) Strategy"
+  ("_ \<rightarrow> _ where _") where 
+  "s1 \<rightarrow> s2 where s3 \<equiv> s1?; wheref s3; s2!"
 
 subsection "Rewrite Semantics"
 
@@ -139,11 +87,7 @@ fun eval :: "('a, 'b, 'c) Strategy \<Rightarrow> ('a) State \<Rightarrow> ('a St
 
 end
 
-
-fun chain_list :: "'b \<Rightarrow> ('a \<Rightarrow> 'b \<Rightarrow> ('b \<times> 'c)) \<Rightarrow> 'a list \<Rightarrow> ('b \<times> 'c list)" where
-  "chain_list a f [] = (a, [])" |
-  "chain_list a f (x # xs) =
-    (let (a', x') = f x a in
-    (let (a'', xs') = (chain_list a' f xs) in (a'', x' # xs')))"
+notation plus (infixl "+" 65)
+notation less ("(_/ < _)"  [51, 51] 50)
 
 end
